formal/inference/Increment_Reset.thy
@@ -20,7 +20,7 @@ fun insert_increment :: update_modifier where
           newReg = R r;
           newT1 = \<lparr>Label = Label t1, Arity = Arity t1, Guard = [], Outputs = [Plus (V newReg) (V (I 1))], Updates=((newReg, Plus (V newReg) (V (I 1)))#Updates t1)\<rparr>;
           newT2 = \<lparr>Label = Label t2, Arity = Arity t2, Guard = [], Outputs = [Plus (V newReg) (V (I 1))], Updates=((newReg, Plus (V newReg) (V (I 1)))#Updates t2)\<rparr>;
-          initialised = fimage (\<lambda>(uid, (from, to), t). (uid, (from, to), (if (to = arrives t1ID new \<or> to = arrives t2ID new) \<and> t \<noteq> t1 \<and> t \<noteq> t2 then initialiseReg t newReg else t))) new 
+          initialised = fimage (\<lambda>(uid, (from, to), t). (uid, (from, to), (if (to = dest t1ID new \<or> to = dest t2ID new) \<and> t \<noteq> t1 \<and> t \<noteq> t2 then initialiseReg t newReg else t))) new 
           in 
           Some (replaceAll (replaceAll initialised t2 newT2) t1 newT1)
      else
