formal/clean.sh
@@ -1,1 +1,0 @@
-find . -name "*thy~" -exec rm {} ;
